compilerProofScript.sml
@@ -1,0 +1,67 @@
+Theory compilerProof
+Ancestors
+  panLang panProps panSem compiler p4 p4_bigstep p4_exec_sem
+Libs
+  wordsLib
+
+
+(*----NOTESs----*)
+(*
+Type scope = ``:((varn, (v # lval option)) alist)``;
+Type state = 
+    <| locals      : varname |-> 'a v
+     ; globals     : varname |-> 'a v
+e     ; code        : funname |-> ((varname # shape) list # ('a panLang$prog))
+                     (* arguments (with shape), body *)
+     ; eshapes     : eid |-> shape
+     ; memory      : 'a word -> 'a word_lab
+     ; memaddrs    : ('a word) set
+     ; sh_memaddrs : ('a word) set
+     ; clock       : num
+     ; be          : bool
+     ; ffi         : 'ffi ffi_state
+     ; base_addr   : 'a word
+     ; top_addr    : 'a word;          
+
+val s = ``(s:('a,'ffi) panSem$state)``
+*)
+
+(*----VERIFICATIONS----*)
+  
+(* Semantic properties of the value-relations *)
+Inductive v_rel:
+  v_rel (e_v (v_bool T)) (Val (Word 1w)) ∧
+  v_rel (e_v (v_bool F)) (Val (Word 0w)) ∧
+  (v_rel (e_v (v_bit (b,l))) (Val (Word wrd)) ∧ MAP (\(x,y).case (x,y) of (T,1) => T | (F,0) => T | (_,_) => F) $ ZIP (b,word_to_bin_list (wrd:word64)))
+End
+
+Theorem compile_exp_correct:
+  (∀ e uninit (scope_lists:scope_list) e' (n:num) m pan_e s.
+    bigstep_e_exec uninit (scope_lists:scope_list) (INL (e)) (n:num) = SOME $ (INL e', m) ∧
+    is_v e' ∧ compile_exp e = SOME pan_e ∧ state_rel scope_lists s ⇒
+    ∃ v. eval s pan_e = SOME v ∧
+         v_rel e' v ) ∧
+  ∀ es uninit (scope_lists:scope_list) es' (n:num) m pan_es s.
+    bigstep_e_exec uninit (scope_lists:scope_list) (INR (es)) (n:num) = SOME $ (INR es', m) ∧
+    EVERY is_v es' ∧ OPT_MMAP compile_exp es = SOME pan_es ∧ state_rel scope_lists s ⇒
+    ∃ vs. OPT_MMAP (eval s) pan_es = SOME vs ∧
+         LIST_REL v_rel es' vs                  
+Proof
+  Induct
+  >~ [‘e_v _’]
+  >- (rw [compile_exp_def, bigstep_e_exec_def, AllCaseEqs()] >> rw [eval_def] >> metis_tac [v_rel_rules])
+  >~ [‘e_unop _’]
+  >- rw [compile_unop_def, compile_exp_def, bigstep_e_exec_def, AllCaseEqs()]
+  >> (gvs[oneline e_exec_unop_def, AllCaseEqs(), oneline unop_exec_def] >> first_x_assum drule_all >> strip_tac >> rw[eval_def] >> gvs[v_rel_cases] >> gvs[wordLangTheory.word_op_def] >> gvs[wordLangTheory.word_op_def])
+  >> (gvs[oneline e_exec_unop_def, AllCaseEqs(), oneline unop_exec_def] >> first_x_assum drule_all >> strip_tac >> rw[eval_def] >> gvs[v_rel_cases] >> fs[bitv_unop_def] >> gvs[wordLangTheory.word_op_def])
+  >> (gvs[oneline e_exec_unop_def, AllCaseEqs(), oneline unop_exec_def] >> first_x_assum drule_all >> strip_tac >> rw[eval_def] >> gvs[v_rel_cases] >> fs[bitv_unop_def, AllCaseEqs()] >> gvs[wordLangTheory.word_op_def] >> gvs[v_rel_cases])
+  >> (gvs[oneline e_exec_unop_def, AllCaseEqs(), oneline unop_exec_def] >> first_x_assum drule_all >> strip_tac >> rw[eval_def] >> gvs[v_rel_cases] >> gvs[wordLangTheory.word_op_def])
+  >> (gvs[oneline e_exec_unop_def, AllCaseEqs(), oneline unop_exec_def] >> rw[eval_def] >> gvs[v_rel_cases] >> gvs[]
+  >~ [‘e_binop _’]
+  >- cheat
+  >~ [‘INR []’]
+  >- (rw [bigstep_e_exec_def])
+  >~ [‘INR (_::_)’]
+  >- cheat >>
+  gvs [compile_exp_def]
+QED
